Tactic_Inline.thy
@@ -98,15 +98,20 @@ lemma filter_local_empty: "filter_local {} == {}"
 
 lemma local_variable_name_renaming_same: 
   "local_variable_name_renaming ((a,b)#X) (mk_variable_untyped (LVariable a :: 'a::prog_type variable))
-      == mk_variable_untyped (LVariable b :: 'a variable)"
-  by later
+      == local_variable_name_renaming X (mk_variable_untyped (LVariable b :: 'a variable))"
+  by (subst Rep_rename_local_variables_var[symmetric], simp)
 
-(* TODO how to make the simplifier use this? *)
+lemma local_variable_name_renaming_id: 
+  "local_variable_name_renaming [] x == x"
+  unfolding local_variable_name_renaming_def by simp
+
 lemma local_variable_name_renaming_notsame: 
   assumes "a\<noteq>x" and "b\<noteq>x"
   shows "local_variable_name_renaming ((a,b)#X) (mk_variable_untyped (LVariable x :: 'a::prog_type variable))
-      == mk_variable_untyped (LVariable x :: 'a variable)"
-  by later
+      == local_variable_name_renaming X (mk_variable_untyped (LVariable x :: 'a variable))"
+  apply (subst Rep_rename_local_variables_var[symmetric])
+  apply (subst rename_local_variables_var_notsame)
+  using assms by simp_all
 
 lemmas callproc_conditions_simp =  
   filter_global' filter_global'_cons1 filter_global'_cons2
@@ -116,19 +121,47 @@ lemmas callproc_conditions_simp =
   local_variable_name_renaming_nil local_variable_name_renaming_same image_empty[THEN eq_reflection]
   vars_unit_pattern[THEN eq_reflection] vars_pair_pattern[THEN eq_reflection] 
   append_Cons[THEN eq_reflection] append_Nil[THEN eq_reflection]
-  rename_local_variables_pattern_id[THEN eq_reflection]
+  rename_local_variables_pattern_id[THEN eq_reflection] local_variable_name_renaming_id
   local_variable_name_renaming_set local_variable_name_renaming_cons 
   local_variable_name_renaming_nil2 local_variable_name_renaming_notsame
+
+(* TODO remove *)
+ML {*
+@{context} |> Raw_Simplifier.simpset_of |> dest_ss
+*}
+
+(* TODO remove *)
+ML {*
+val subgoaler_simpset = @{context} 
+|> put_simpset HOL_basic_ss
+|> (fn x => x addsimps @{thms List.list.inject String.char.inject String.nibble.distinct HOL.simp_thms})
+|> Raw_Simplifier.simpset_of
+
+val ss = @{context} 
+|> put_simpset HOL_basic_ss 
+|> (fn x => x addsimps @{thms filter_global' filter_global'_cons1 filter_global'_cons2
+  filter_global'_nil filter_local_union filter_local' vars_variable_pattern[THEN eq_reflection]
+  filter_local'_cons1 filter_local'_cons2 filter_local'_nil filter_local_insert1
+  filter_local_empty local_variable_name_renaming_insert local_variable_name_renaming_union
+  local_variable_name_renaming_nil local_variable_name_renaming_same image_empty[THEN eq_reflection]
+  vars_unit_pattern[THEN eq_reflection] vars_pair_pattern[THEN eq_reflection] 
+  append_Cons[THEN eq_reflection] append_Nil[THEN eq_reflection]
+  rename_local_variables_pattern_id[THEN eq_reflection] local_variable_name_renaming_id
+  local_variable_name_renaming_set local_variable_name_renaming_cons 
+  local_variable_name_renaming_nil2 local_variable_name_renaming_notsame
+})
+|> Simplifier.set_subgoaler (fn ctx => (@{print} "init_subgoaler"; simp_tac (put_simpset subgoaler_simpset ctx)))
+|> Raw_Simplifier.simpset_of
+*}
+
 
 (* TODO remove *)
 lemma 
   "local_variable_name_renaming [(''a'',''b'')] (mk_variable_untyped (LVariable ''x'' :: int variable))
   = mk_variable_untyped (LVariable ''x'' :: int variable)"
-using[[simp_trace_new]]
-apply (simp add: callproc_conditions_simp)
-SORRY
+using[[simp_trace, simp_trace_depth_limit=4]]
+by (tactic \<open>simp_tac (put_simpset ss @{context}) 1\<close>) 
 
-find_theorems "_ ` set _"
 end
 
 ML_file "tactic_inline.ML"
